Tried doing a top down approach with the paint operator, does not look promisisng, may need to abstract away exchange and contraction with lists instead of formula structure.

theories/Logic/paint.v
@@ -6,62 +6,58 @@ From Cyclic_PA.Logic Require Import fol.
 Require Import List.
 Import ListNotations.
 
-Inductive subst_ind : Type :=
-| ind_0 : subst_ind
-| ind_1 : subst_ind
-| lor_ind : subst_ind -> subst_ind -> subst_ind.
+Inductive paint_ind : Type :=
+| colour : list nat -> paint_ind
+| lor_ind : paint_ind -> paint_ind -> paint_ind.
 
-Notation "(0)" := ind_0.
-Notation "(1)" := ind_1.
-Notation "( x y )" := (lor_ind x y).
+Notation "( 0 )" := (colour [0]).
+Notation "( 1 )" := (colour [1]).
+Notation "< L |" := (colour L).
+Notation "< x , y |" := (lor_ind x y).
+
+Section Paint.
 
 Lemma subst_eq_dec :
-    forall (S1 S2 : subst_ind),
+    forall (S1 S2 : paint_ind),
         {S1 = S2} + {S1 <> S2}.
 Proof.
 induction S1;
 destruct S2.
-1,5 : apply (left eq_refl).
-1-6 : right; discriminate.
-case (IHS1_1 S2_1) as [EQ1 | NE1].
-case (IHS1_2 S2_2) as [EQ2 | NE2].
-- left.
-  rewrite EQ1,EQ2.
-  reflexivity.
-- right.
-  intros FAL.
-  apply NE2.
-  inversion FAL.
-  reflexivity.
-- right.
-  intros FAL.
-  apply NE1.
-  inversion FAL.
-  reflexivity.
+case (list_eq_dec nat_eq_dec l l0) as [[] | NE].
+1 : apply (left eq_refl).
+2-3 : right; discriminate.
+2 : case (IHS1_1 S2_1) as [EQ1 | NE].
+2 : case (IHS1_2 S2_2) as [EQ2 | NE].
+2 : { left.
+      rewrite EQ1,EQ2.
+      reflexivity. }
+all : right;
+      intros FAL;
+      apply NE;
+      inversion FAL;
+      reflexivity.
 Qed.
 
-Fixpoint non_target (A : formula) : subst_ind :=
+Fixpoint coat (A : formula) (L : list nat) : paint_ind :=
 match A with
-| lor B C => lor_ind (non_target B) (non_target C)
-| _ => (0)
+| lor B C => lor_ind (coat B L) (coat C L)
+| _ => <L|
 end.
 
-Fixpoint target (A : formula) : subst_ind :=
-match A with
-| lor B C => lor_ind (target B) (target C)
-| _ => (1)
-end.
+Definition non_target (A : formula) := coat A [0].
 
-Fixpoint subst_ind_fit (A : formula) (S : subst_ind) : bool :=
+Definition target (A : formula) := coat A [1].
+
+Fixpoint paint_ind_fit (A : formula) (S : paint_ind) : bool :=
 match A, S with
 | lor B C, lor_ind S_B S_C =>
-    subst_ind_fit B S_B && subst_ind_fit C S_C
+    paint_ind_fit B S_B && paint_ind_fit C S_C
 | _, lor_ind _ _ => false
 | lor _ _, _ => false
 | _, _ => true
 end.
 
-Fixpoint formula_sub_ind_fit (A D E : formula) (S : subst_ind) : formula :=
+Fixpoint formula_sub_ind_fit (A D E : formula) (S : paint_ind) : formula :=
 match A with
 | lor B C =>
   (match S with
@@ -76,15 +72,15 @@ match A with
   end)
 end.
 
-Definition formula_sub_ind (A D E : formula) (S : subst_ind) : formula :=
-match subst_ind_fit A S with
+Definition formula_sub_ind (A D E : formula) (S : paint_ind) : formula :=
+match paint_ind_fit A S with
 | false => A
 | true => formula_sub_ind_fit A D E S
 end.
 
 Lemma sub_fit_true :
-    forall (A D E : formula) (S : subst_ind),
-        subst_ind_fit A S = true ->
+    forall (A D E : formula) (S : paint_ind),
+        paint_ind_fit A S = true ->
             formula_sub_ind A D E S = formula_sub_ind_fit A D E S.
 Proof.
 intros A D E S FS.
@@ -95,8 +91,8 @@ reflexivity.
 Qed.
 
 Lemma sub_fit_false :
-    forall (A D E : formula) (S : subst_ind),
-        subst_ind_fit A S = false ->
+    forall (A D E : formula) (S : paint_ind),
+        paint_ind_fit A S = false ->
             formula_sub_ind A D E S = A.
 Proof.
 intros A D E S FS.
@@ -124,7 +120,7 @@ Lemma formula_sub_ind_0 :
         formula_sub_ind A D E (0) = A.
 Proof.
 intros A D E.
-case (subst_ind_fit A (0)) eqn:HA;
+case (paint_ind_fit A (0)) eqn:HA;
 unfold formula_sub_ind;
 rewrite HA.
 - rewrite formula_sub_ind_fit_0.
@@ -133,8 +129,8 @@ rewrite HA.
 Qed.
 
 Lemma formula_sub_ind_lor :
-    forall (A B D E : formula) (S_A S_B : subst_ind),
-        subst_ind_fit A S_A && subst_ind_fit B S_B = true ->
+    forall (A B D E : formula) (S_A S_B : paint_ind),
+        paint_ind_fit A S_A && paint_ind_fit B S_B = true ->
             formula_sub_ind (lor A B) D E (lor_ind S_A S_B) = 
                 lor (formula_sub_ind A D E S_A) (formula_sub_ind B D E S_B).
 Proof.
@@ -142,40 +138,43 @@ intros A B D E S_A S_B FS.
 unfold formula_sub_ind.
 destruct (and_bool_prop _ _ FS) as [FSA FSB].
 rewrite FSA,FSB.
-unfold subst_ind_fit; fold subst_ind_fit.
+unfold paint_ind_fit; fold paint_ind_fit.
 rewrite FS.
 unfold formula_sub_ind_fit; fold formula_sub_ind_fit.
 reflexivity.
 Qed.
 
-Lemma non_target_fit :
-    forall (A : formula),
-        subst_ind_fit A (non_target A) = true.
+Lemma coat_fit :
+    forall {A : formula} {L : list nat},
+        paint_ind_fit A (coat A L) = true.
 Proof.
-intros A.
-unfold subst_ind_fit, non_target.
+intros A L.
+unfold paint_ind_fit, coat.
 induction A.
 3 : rewrite IHA1, IHA2.
 all : reflexivity.
+Qed.
+
+Lemma non_target_fit :
+    forall {A : formula},
+        paint_ind_fit A (non_target A) = true.
+Proof.
+intros A. apply coat_fit.
 Qed.
 
 Lemma target_fit :
-    forall (A : formula),
-        subst_ind_fit A (target A) = true.
+    forall {A : formula},
+        paint_ind_fit A (target A) = true.
 Proof.
-intros A.
-unfold subst_ind_fit, target.
-induction A.
-3 : rewrite IHA1, IHA2.
-all : reflexivity.
+intros A. apply coat_fit.
 Qed.
 
 Lemma non_target_sub_fit :
-    forall (A : formula) (n : nat) (t : term),
-        subst_ind_fit (substitution A n t) (non_target A) = true.
+    forall {A : formula} {n : nat} {t : term},
+        paint_ind_fit (substitution A n t) (non_target A) = true.
 Proof.
 intros A n t.
-unfold subst_ind_fit, non_target, substitution.
+unfold paint_ind_fit, non_target, coat, substitution.
 induction A.
 3 : rewrite IHA1, IHA2.
 4 : case (nat_eqb n0 n).
@@ -183,11 +182,11 @@ all : reflexivity.
 Qed.
 
 Lemma target_sub_fit :
-    forall (A : formula) (n : nat) (t : term),
-        subst_ind_fit (substitution A n t) (target A) = true.
+    forall {A : formula} {n : nat} {t : term},
+        paint_ind_fit (substitution A n t) (target A) = true.
 Proof.
 intros A n t.
-unfold subst_ind_fit, target, substitution.
+unfold paint_ind_fit, target, coat, substitution.
 induction A.
 3 : rewrite IHA1, IHA2.
 4 : case (nat_eqb n0 n).
@@ -200,8 +199,9 @@ Lemma non_target_sub' :
 Proof.
 intros A D E.
 induction A;
-unfold non_target, formula_sub_ind_fit;
-fold non_target formula_sub_ind_fit.
+unfold non_target, coat, formula_sub_ind_fit;
+fold coat formula_sub_ind_fit;
+try fold (non_target A1) (non_target A2).
 4 : case (form_eqb (univ n A) D).
 3 : rewrite IHA1, IHA2.
 2 : case (form_eqb (neg A) D).
@@ -219,69 +219,52 @@ rewrite non_target_fit.
 apply non_target_sub'.
 Qed.
 
-Lemma non_target_sub_lor :
-    forall (A B D E : formula) (S : subst_ind),
+Lemma non_target_sub_lor_left :
+    forall (A B D E : formula) (S : paint_ind),
         formula_sub_ind (lor A B) D E (lor_ind (non_target A) S) =
             lor A (formula_sub_ind B D E S).
 Proof.
 intros A B D E S.
-unfold formula_sub_ind, subst_ind_fit, formula_sub_ind_fit;
-fold subst_ind_fit formula_sub_ind_fit.
+unfold formula_sub_ind, paint_ind_fit, formula_sub_ind_fit;
+fold paint_ind_fit formula_sub_ind_fit.
 rewrite non_target_fit, non_target_sub'.
-case (subst_ind_fit B S) eqn:HB;
+case (paint_ind_fit B S) eqn:HB;
 reflexivity.
 Qed.
 
-Lemma non_target_term_sub :
-    forall (A : formula) (n : nat) (t : term),
-        non_target A = non_target (substitution A n t).
+Lemma coat_subst_eq :
+    forall {A : formula} {L : list nat} {n : nat} {t : term},
+        coat (substitution A n t) L = coat A L.
 Proof.
-intros A n t.
+intros A L n t.
 induction A;
-unfold non_target, substitution;
-fold non_target substitution.
+unfold coat, substitution;
+fold coat substitution.
 3 : rewrite IHA1,IHA2.
 4 : case (nat_eqb n0 n).
 all : reflexivity.
 Qed.
 
-Lemma target_term_sub :
+Lemma non_target_subst_eq :
     forall (A : formula) (n : nat) (t : term),
-        target A = target (substitution A n t).
+        non_target (substitution A n t) = non_target A.
 Proof.
 intros A n t.
-induction A;
-unfold target, substitution;
-fold target substitution.
-3 : rewrite IHA1,IHA2.
-4 : case (nat_eqb n0 n).
-all : reflexivity.
+apply coat_subst_eq.
 Qed.
 
-
-Lemma non_target_sub_term' :
-    forall (A C D: formula) (n : nat) (t : term),
-        formula_sub_ind_fit (substitution A n t) C D (non_target A) = (substitution A n t).
+Lemma target_subst_eq :
+    forall (A : formula) (n : nat) (t : term),
+        target (substitution A n t) = target A.
 Proof.
-intros.
-rewrite (non_target_term_sub _ n t).
-apply non_target_sub'.
-Qed.
-
-
-Lemma non_target_sub_term :
-    forall (A C D: formula) (n : nat) (t : term),
-        formula_sub_ind (substitution A n t) C D (non_target A) = (substitution A n t).
-Proof.
-intros.
-rewrite (non_target_term_sub _ n t).
-apply non_target_sub.
+intros A n t.
+apply coat_subst_eq.
 Qed.
 
 Lemma formula_sub_ind_free_list :
     forall (A B C : formula),
         (free_list B = free_list C) ->
-            forall (S : subst_ind),
+            forall (S : paint_ind),
                 free_list (formula_sub_ind_fit A B C S) = free_list A.
 Proof.
 intros A B C FREE.
@@ -292,21 +275,21 @@ unfold formula_sub_ind.
 all : unfold formula_sub_ind_fit;
       fold formula_sub_ind_fit;
       try case form_eqb eqn:EQ;
-      destruct S;
+      destruct S as [[ | [ | [ | ] ] [ | ] ] | ];
       try apply form_eqb_eq in EQ;
       try destruct EQ, FREE;
       try reflexivity.
 
 1 : unfold free_list;
-    fold free_list.
-    rewrite IHA1,IHA2.
+    fold free_list;
+    rewrite IHA1,IHA2;
     reflexivity.
 Qed.
 
 Lemma formula_sub_ind_free_list_sub :
     forall (A B C : formula),
         (incl (free_list C) (free_list B)) ->
-            forall (S : subst_ind),
+            forall (S : paint_ind),
                 incl (free_list (formula_sub_ind_fit A B C S)) (free_list A).
 Proof.
 intros A B C FREE.
@@ -316,7 +299,7 @@ unfold formula_sub_ind.
 
 all : unfold formula_sub_ind_fit in IN;
       try case form_eqb eqn:EQ;
-      destruct S;
+      destruct S as [[ | [ | [ | ] ] [ | ] ] | ];
       try apply form_eqb_eq in EQ;
       fold formula_sub_ind_fit in IN;
       try destruct EQ;
@@ -336,36 +319,35 @@ Lemma formula_sub_ind_closed :
     forall (A B C : formula),
         closed A = true ->
             (closed B = true -> closed C = true) ->
-                forall (S : subst_ind),
+                forall (S : paint_ind),
                     closed (formula_sub_ind A B C S) = true.
 Proof.
 intros A B C.
 induction A;
 intros CA CBC S;
 unfold formula_sub_ind.
-4 : case (subst_ind_fit (univ n A) S).
-3 : case (subst_ind_fit (lor A1 A2) S) eqn:FS.
-2 : case (subst_ind_fit (neg A) S).
-1 : case (subst_ind_fit (atom a) S).
+4 : case (paint_ind_fit (univ n A) S).
+3 : case (paint_ind_fit (lor A1 A2) S) eqn:FS.
+2 : case (paint_ind_fit (neg A) S).
+1 : case (paint_ind_fit (atom a) S).
 all : try apply CA;
       unfold formula_sub_ind_fit;
       fold formula_sub_ind_fit;
-      destruct S;
-      try apply CA.
-7 : { unfold formula_sub_ind, formula_sub_ind_fit, subst_ind_fit, closed in *;
-      fold formula_sub_ind formula_sub_ind_fit subst_ind_fit closed in *.
-      destruct (and_bool_prop _ _ CA) as [CA1 CA2].
-      destruct (and_bool_prop _ _ FS) as [FS1 FS2].
-      pose proof (IHA1 CA1 CBC S1) as CFA1.
-      rewrite FS1 in CFA1.
-      rewrite CFA1.
-      pose proof (IHA2 CA2 CBC S2) as CFA2.
-      rewrite FS2 in CFA2.
-      rewrite CFA2.
-      reflexivity. }
-7-9 : case (form_eqb (univ n A) B) eqn:EQ.
-4-6 : case (form_eqb (neg A) B) eqn:EQ.
-1-3 : case (form_eqb (atom a) B) eqn:EQ.
+      destruct S as [[ | [ | [ | ] ] [ | ] ] | ].
+24 : { unfold formula_sub_ind, formula_sub_ind_fit, paint_ind_fit, closed in *;
+       fold formula_sub_ind formula_sub_ind_fit paint_ind_fit closed in *.
+       destruct (and_bool_prop _ _ CA) as [CA1 CA2].
+       destruct (and_bool_prop _ _ FS) as [FS1 FS2].
+       pose proof (IHA1 CA1 CBC S1) as CFA1.
+       rewrite FS1 in CFA1.
+       rewrite CFA1.
+       pose proof (IHA2 CA2 CBC S2) as CFA2.
+       rewrite FS2 in CFA2.
+       rewrite CFA2.
+       reflexivity. }
+24-31 : case (form_eqb (univ n A) B) eqn:EQ.
+9-16 : case (form_eqb (neg A) B) eqn:EQ.
+1-8 : case (form_eqb (atom a) B) eqn:EQ.
 all : try apply CA;
       apply form_eqb_eq in EQ;
       destruct EQ;
@@ -374,12 +356,12 @@ Qed.
 
 Lemma formula_sub_ind_1 :
     forall (A B : formula),
-        (subst_ind_fit A (1) = true) ->
+        (paint_ind_fit A (1) = true) ->
             formula_sub_ind A A B (1) = B.
 Proof.
 intros A B FS.
 destruct A;
-unfold formula_sub_ind, subst_ind_fit, formula_sub_ind_fit.
+unfold formula_sub_ind, paint_ind_fit, formula_sub_ind_fit.
 3 : inversion FS.
 all : rewrite form_eqb_refl;
       reflexivity.
@@ -387,7 +369,7 @@ Qed.
 
 Theorem lor_sub_right:
     forall C A E,
-        (subst_ind_fit A (1) = true) ->
+        (paint_ind_fit A (1) = true) ->
             formula_sub_ind (lor C A) A E (lor_ind (non_target C) (1)) = lor C E.
 Proof.
 intros C A E FS.
@@ -401,7 +383,7 @@ Qed.
 
 Theorem lor_sub_left:
     forall A D E,
-        (subst_ind_fit A (1) = true) ->
+        (paint_ind_fit A (1) = true) ->
             formula_sub_ind (lor A D) A E (lor_ind (1) (non_target D)) = lor E D.
 Proof.
 intros A D E FS.
@@ -412,3 +394,60 @@ rewrite formula_sub_ind_lor.
 - rewrite FS.
   apply non_target_fit.
 Qed.
+
+Definition paint_ex_ab (I : paint_ind) : paint_ind :=
+match I with
+| <Ia, Ib| => <Ib, Ia|
+| _ => I
+end.
+
+Definition paint_ex_cab (I : paint_ind) : paint_ind :=
+match I with
+| <<Ic, Ia|, Ib| => <<Ic, Ib|, Ia|
+| _ => I
+end.
+
+Definition paint_ex_abd (I : paint_ind) : paint_ind :=
+match I with
+| <<Ia, Ib|, Id| => <<Ib, Ia|, Id|
+| _ => I
+end.
+
+Definition paint_ex_cabd (I : paint_ind) : paint_ind :=
+match I with
+| <<<Ic, Ia|, Ib|, Id| => <<<Ic, Ib|, Ia|, Id|
+| _ => I
+end.
+
+Definition paint_con_a (I : paint_ind) : paint_ind :=
+match I with
+| <Ia, Ib| => match subst_eq_dec Ia Ib with
+    | True => Ia
+    end
+| _ => I
+end.
+
+Definition paint_con_ad (I : paint_ind) : paint_ind :=
+match I with
+| <<Ia, Ib|, Id| => match subst_eq_dec Ia Ib with
+    | True => <Ia, Id|
+    end
+| _ => I
+end.
+
+Definition paint_dem_ab (I1 I2 : paint_ind) : paint_ind :=
+match I1,I2 with 
+| colour L1, colour L2 => <L1 ++ L2|
+| _, _ => I1
+end.
+
+Definition paint_dem_abd (I1 I2 : paint_ind) : paint_ind :=
+match I1,I2 with 
+| <colour L1, Ic|, <colour L2, Id| => match subst_eq_dec Ic Id with
+    | True => <<L1 ++ L2|, Id|
+    end
+| _, _ => I1
+end.
+
+
+End Paint.
