theories/Logic/PA_cyclic.v
@@ -11,6 +11,7 @@ From Cyclic_PA.Maths Require Import ordinals.
 
 From Cyclic_PA.Logic Require Import definitions.
 From Cyclic_PA.Logic Require Import fol.
+From Cyclic_PA.Logic Require Import paint.
 
 Import ListNotations.
 
@@ -109,7 +110,7 @@ Inductive PA_cyclic_pre : formula -> nat -> ord -> list formula -> Type :=
 | loop2 : forall {C A : formula} {n : nat} {d1 d2 : nat} {alpha1 alpha2 : ord} (L1 L2 : list formula),
     In n (free_list A) ->
     PA_cyclic_pre (lor C (substitution A n zero)) d1 alpha1 L1 ->
-    PA_cyclic_pre (lor C (substitution A n (succ (var n)))) d2 alpha2 ((lor C A) :: L2) ->
+    PA_cyclic_pre (lor C (substitution A n (succ (var n)))) d2 alpha2 (A :: L2) ->
     PA_cyclic_pre (lor C (univ n A)) (max d1 d2) (ord_succ (ord_add alpha1 (ord_mult alpha2 (wcon (wcon Zero 0 Zero) 0 Zero)))) (L2 ++ L1)
 
 | cut1 : forall (C A : formula) {d1 d2 : nat} {alpha1 alpha2 : ord} {L1 L2 : list formula},
